chore(MPL): update smithy files for new keyrings (#76)
Co-authored-by: Andrew Jewell <107044381+ajewellamz@users.noreply.github.com>
Co-authored-by: Lucas McDonald <lucasmcdonald3@gmail.com>

AwsCryptographicMaterialProviders/runtimes/java/src/main/smithy-generated/software/amazon/cryptography/materialproviders/MaterialProviders.java
@@ -17,6 +17,7 @@ import software.amazon.cryptography.materialproviders.internaldafny.types.IAwsCr
 import software.amazon.cryptography.materialproviders.model.AlgorithmSuiteInfo;
 import software.amazon.cryptography.materialproviders.model.CreateAwsKmsDiscoveryKeyringInput;
 import software.amazon.cryptography.materialproviders.model.CreateAwsKmsDiscoveryMultiKeyringInput;
+import software.amazon.cryptography.materialproviders.model.CreateAwsKmsEcdhKeyringInput;
 import software.amazon.cryptography.materialproviders.model.CreateAwsKmsHierarchicalKeyringInput;
 import software.amazon.cryptography.materialproviders.model.CreateAwsKmsKeyringInput;
 import software.amazon.cryptography.materialproviders.model.CreateAwsKmsMrkDiscoveryKeyringInput;
@@ -30,6 +31,7 @@ import software.amazon.cryptography.materialproviders.model.CreateDefaultClientS
 import software.amazon.cryptography.materialproviders.model.CreateDefaultCryptographicMaterialsManagerInput;
 import software.amazon.cryptography.materialproviders.model.CreateMultiKeyringInput;
 import software.amazon.cryptography.materialproviders.model.CreateRawAesKeyringInput;
+import software.amazon.cryptography.materialproviders.model.CreateRawEcdhKeyringInput;
 import software.amazon.cryptography.materialproviders.model.CreateRawRsaKeyringInput;
 import software.amazon.cryptography.materialproviders.model.CreateRequiredEncryptionContextCMMInput;
 import software.amazon.cryptography.materialproviders.model.DecryptionMaterials;
@@ -103,6 +105,25 @@ public class MaterialProviders {
       software.amazon.cryptography.materialproviders.internaldafny.types.IKeyring,
       Error
     > result = this._impl.CreateAwsKmsDiscoveryMultiKeyring(dafnyValue);
+    if (result.is_Failure()) {
+      throw ToNative.Error(result.dtor_error());
+    }
+    return Keyring.wrap(result.dtor_value());
+  }
+
+  /**
+   * Creates an AWS KMS ECDH Keyring, which wraps and unwraps datakeys by deriving a shared data key from the established shared secret between parties through the ECDH protocol.
+   *
+   * @param input Inputs for creating a AWS KMS ECDH Keyring.
+   * @return Outputs for creating a Keyring.
+   */
+  public IKeyring CreateAwsKmsEcdhKeyring(CreateAwsKmsEcdhKeyringInput input) {
+    software.amazon.cryptography.materialproviders.internaldafny.types.CreateAwsKmsEcdhKeyringInput dafnyValue =
+      ToDafny.CreateAwsKmsEcdhKeyringInput(input);
+    Result<
+      software.amazon.cryptography.materialproviders.internaldafny.types.IKeyring,
+      Error
+    > result = this._impl.CreateAwsKmsEcdhKeyring(dafnyValue);
     if (result.is_Failure()) {
       throw ToNative.Error(result.dtor_error());
     }
@@ -355,6 +376,25 @@ public class MaterialProviders {
       software.amazon.cryptography.materialproviders.internaldafny.types.IKeyring,
       Error
     > result = this._impl.CreateRawAesKeyring(dafnyValue);
+    if (result.is_Failure()) {
+      throw ToNative.Error(result.dtor_error());
+    }
+    return Keyring.wrap(result.dtor_value());
+  }
+
+  /**
+   * Creates a Raw ECDH Keyring, which wraps and unwraps datakeys by deriving a shared data key from the established shared secret between parties through the ECDH protocol.
+   *
+   * @param input Inputs for creating a raw ECDH Keyring.
+   * @return Outputs for creating a Keyring.
+   */
+  public IKeyring CreateRawEcdhKeyring(CreateRawEcdhKeyringInput input) {
+    software.amazon.cryptography.materialproviders.internaldafny.types.CreateRawEcdhKeyringInput dafnyValue =
+      ToDafny.CreateRawEcdhKeyringInput(input);
+    Result<
+      software.amazon.cryptography.materialproviders.internaldafny.types.IKeyring,
+      Error
+    > result = this._impl.CreateRawEcdhKeyring(dafnyValue);
     if (result.is_Failure()) {
       throw ToNative.Error(result.dtor_error());
     }
