AwsCryptographicMaterialProviders/runtimes/java/src/main/smithy-generated/software/amazon/cryptography/materialproviders/model/CreateRawEcdhKeyringInput.java
@@ -1,0 +1,121 @@
+// Copyright Amazon.com Inc. or its affiliates. All Rights Reserved.
+// SPDX-License-Identifier: Apache-2.0
+// Do not modify this file. This file is machine generated, and any changes to it will be overwritten.
+package software.amazon.cryptography.materialproviders.model;
+
+import java.util.Objects;
+
+/**
+ * Inputs for creating a raw ECDH Keyring.
+ */
+public class CreateRawEcdhKeyringInput {
+
+  /**
+   * The Key Agreement Scheme configuration that is responsible for how the shared secret is calculated.
+   */
+  private final RawEcdhStaticConfigurations KeyAgreementScheme;
+
+  /**
+   * The named curve that corresponds to the curve on which the sender's private and recipient's public key lie.
+   */
+  private final EccCurveSpec curveSpec;
+
+  protected CreateRawEcdhKeyringInput(BuilderImpl builder) {
+    this.KeyAgreementScheme = builder.KeyAgreementScheme();
+    this.curveSpec = builder.curveSpec();
+  }
+
+  /**
+   * @return The Key Agreement Scheme configuration that is responsible for how the shared secret is calculated.
+   */
+  public RawEcdhStaticConfigurations KeyAgreementScheme() {
+    return this.KeyAgreementScheme;
+  }
+
+  /**
+   * @return The named curve that corresponds to the curve on which the sender's private and recipient's public key lie.
+   */
+  public EccCurveSpec curveSpec() {
+    return this.curveSpec;
+  }
+
+  public Builder toBuilder() {
+    return new BuilderImpl(this);
+  }
+
+  public static Builder builder() {
+    return new BuilderImpl();
+  }
+
+  public interface Builder {
+    /**
+     * @param KeyAgreementScheme The Key Agreement Scheme configuration that is responsible for how the shared secret is calculated.
+     */
+    Builder KeyAgreementScheme(RawEcdhStaticConfigurations KeyAgreementScheme);
+
+    /**
+     * @return The Key Agreement Scheme configuration that is responsible for how the shared secret is calculated.
+     */
+    RawEcdhStaticConfigurations KeyAgreementScheme();
+
+    /**
+     * @param curveSpec The named curve that corresponds to the curve on which the sender's private and recipient's public key lie.
+     */
+    Builder curveSpec(EccCurveSpec curveSpec);
+
+    /**
+     * @return The named curve that corresponds to the curve on which the sender's private and recipient's public key lie.
+     */
+    EccCurveSpec curveSpec();
+
+    CreateRawEcdhKeyringInput build();
+  }
+
+  static class BuilderImpl implements Builder {
+
+    protected RawEcdhStaticConfigurations KeyAgreementScheme;
+
+    protected EccCurveSpec curveSpec;
+
+    protected BuilderImpl() {}
+
+    protected BuilderImpl(CreateRawEcdhKeyringInput model) {
+      this.KeyAgreementScheme = model.KeyAgreementScheme();
+      this.curveSpec = model.curveSpec();
+    }
+
+    public Builder KeyAgreementScheme(
+      RawEcdhStaticConfigurations KeyAgreementScheme
+    ) {
+      this.KeyAgreementScheme = KeyAgreementScheme;
+      return this;
+    }
+
+    public RawEcdhStaticConfigurations KeyAgreementScheme() {
+      return this.KeyAgreementScheme;
+    }
+
+    public Builder curveSpec(EccCurveSpec curveSpec) {
+      this.curveSpec = curveSpec;
+      return this;
+    }
+
+    public EccCurveSpec curveSpec() {
+      return this.curveSpec;
+    }
+
+    public CreateRawEcdhKeyringInput build() {
+      if (Objects.isNull(this.KeyAgreementScheme())) {
+        throw new IllegalArgumentException(
+          "Missing value for required field `KeyAgreementScheme`"
+        );
+      }
+      if (Objects.isNull(this.curveSpec())) {
+        throw new IllegalArgumentException(
+          "Missing value for required field `curveSpec`"
+        );
+      }
+      return new CreateRawEcdhKeyringInput(this);
+    }
+  }
+}
