AwsCryptographicMaterialProviders/runtimes/java/src/main/smithy-generated/software/amazon/cryptography/materialproviders/model/PublicKeyDiscoveryInput.java
@@ -1,0 +1,80 @@
+// Copyright Amazon.com Inc. or its affiliates. All Rights Reserved.
+// SPDX-License-Identifier: Apache-2.0
+// Do not modify this file. This file is machine generated, and any changes to it will be overwritten.
+package software.amazon.cryptography.materialproviders.model;
+
+import java.nio.ByteBuffer;
+import java.util.Objects;
+
+/**
+ * Inputs for creating a PublicKeyDiscovery Configuration.
+ */
+public class PublicKeyDiscoveryInput {
+
+  /**
+   * The sender's private key
+   */
+  private final ByteBuffer senderStaticPrivateKey;
+
+  protected PublicKeyDiscoveryInput(BuilderImpl builder) {
+    this.senderStaticPrivateKey = builder.senderStaticPrivateKey();
+  }
+
+  /**
+   * @return The sender's private key
+   */
+  public ByteBuffer senderStaticPrivateKey() {
+    return this.senderStaticPrivateKey;
+  }
+
+  public Builder toBuilder() {
+    return new BuilderImpl(this);
+  }
+
+  public static Builder builder() {
+    return new BuilderImpl();
+  }
+
+  public interface Builder {
+    /**
+     * @param senderStaticPrivateKey The sender's private key
+     */
+    Builder senderStaticPrivateKey(ByteBuffer senderStaticPrivateKey);
+
+    /**
+     * @return The sender's private key
+     */
+    ByteBuffer senderStaticPrivateKey();
+
+    PublicKeyDiscoveryInput build();
+  }
+
+  static class BuilderImpl implements Builder {
+
+    protected ByteBuffer senderStaticPrivateKey;
+
+    protected BuilderImpl() {}
+
+    protected BuilderImpl(PublicKeyDiscoveryInput model) {
+      this.senderStaticPrivateKey = model.senderStaticPrivateKey();
+    }
+
+    public Builder senderStaticPrivateKey(ByteBuffer senderStaticPrivateKey) {
+      this.senderStaticPrivateKey = senderStaticPrivateKey;
+      return this;
+    }
+
+    public ByteBuffer senderStaticPrivateKey() {
+      return this.senderStaticPrivateKey;
+    }
+
+    public PublicKeyDiscoveryInput build() {
+      if (Objects.isNull(this.senderStaticPrivateKey())) {
+        throw new IllegalArgumentException(
+          "Missing value for required field `senderStaticPrivateKey`"
+        );
+      }
+      return new PublicKeyDiscoveryInput(this);
+    }
+  }
+}
