AwsCryptographicMaterialProviders/runtimes/net/Generated/AwsCryptographicMaterialProviders/KmsEcdhStaticConfigurations.cs
@@ -1,0 +1,40 @@
+// Copyright Amazon.com Inc. or its affiliates. All Rights Reserved.
+// SPDX-License-Identifier: Apache-2.0
+// Do not modify this file. This file is machine generated, and any changes to it will be overwritten.
+using System;
+using AWS.Cryptography.MaterialProviders;
+namespace AWS.Cryptography.MaterialProviders
+{
+  public class KmsEcdhStaticConfigurations
+  {
+    private AWS.Cryptography.MaterialProviders.KmsPublicKeyDiscoveryInput _kmsPublicKeyDiscovery;
+    private AWS.Cryptography.MaterialProviders.KmsPrivateKeyToStaticPublicKeyInput _kmsPrivateKeyToStaticPublicKey;
+    public AWS.Cryptography.MaterialProviders.KmsPublicKeyDiscoveryInput KmsPublicKeyDiscovery
+    {
+      get { return this._kmsPublicKeyDiscovery; }
+      set { this._kmsPublicKeyDiscovery = value; }
+    }
+    public bool IsSetKmsPublicKeyDiscovery()
+    {
+      return this._kmsPublicKeyDiscovery != null;
+    }
+    public AWS.Cryptography.MaterialProviders.KmsPrivateKeyToStaticPublicKeyInput KmsPrivateKeyToStaticPublicKey
+    {
+      get { return this._kmsPrivateKeyToStaticPublicKey; }
+      set { this._kmsPrivateKeyToStaticPublicKey = value; }
+    }
+    public bool IsSetKmsPrivateKeyToStaticPublicKey()
+    {
+      return this._kmsPrivateKeyToStaticPublicKey != null;
+    }
+    public void Validate()
+    {
+      var numberOfPropertiesSet = Convert.ToUInt16(IsSetKmsPublicKeyDiscovery()) +
+      Convert.ToUInt16(IsSetKmsPrivateKeyToStaticPublicKey());
+      if (numberOfPropertiesSet == 0) throw new System.ArgumentException("No union value set");
+
+      if (numberOfPropertiesSet > 1) throw new System.ArgumentException("Multiple union values set");
+
+    }
+  }
+}
