AwsCryptographicMaterialProviders/dafny/AwsCryptographicMaterialProviders/Model/key-agreement-scheme.smithy
@@ -1,0 +1,97 @@
+namespace aws.cryptography.materialProviders
+
+use aws.polymorph#javadoc
+
+// Key Agreement Schemes
+
+@enum([
+  {
+    name: "ECC_NIST_P256",
+    value: "secp256r1",
+  },
+  {
+    name: "ECC_NIST_P384",
+    value: "secp384r1",
+  },
+  {
+    name: "ECC_NIST_P521",
+    value: "secp521r1",
+  },
+  {
+    // TODO: come back and double check this is the spec kms uses
+    name: "SM2",
+    value: "SM2PKE",
+  },
+])
+string EccCurveSpec
+
+@javadoc("Supported ECDH KeyAgreement Schemes")
+union KeyAgreementScheme {
+    StaticConfiguration: StaticConfigurations
+}
+
+@javadoc("Supported configurations for the StaticConfiguration Key Agreement Scheme")
+union StaticConfigurations {
+    AWS_KMS_ECDH: KmsEcdhStaticConfigurations,
+    RAW_ECDH: RawEcdhStaticConfigurations
+}
+
+@javadoc("Allowed configurations when using a KmsEcdhStaticConfigurations")
+union KmsEcdhStaticConfigurations {
+    KmsPublicKeyDiscovery: KmsPublicKeyDiscoveryInput,
+    KmsPrivateKeyToStaticPublicKey: KmsPrivateKeyToStaticPublicKeyInput,
+}
+
+@javadoc("List of configurations when using a RawEcdhStaticConfigurations")
+union RawEcdhStaticConfigurations {
+    PublicKeyDiscovery: PublicKeyDiscoveryInput,
+    RawPrivateKeyToStaticPublicKey: RawPrivateKeyToStaticPublicKeyInput,
+    EphemeralPrivateKeyToStaticPublicKey: EphemeralPrivateKeyToStaticPublicKeyInput 
+}
+
+union KmsRecipientConfiguration {
+    RecipientKmsKeyId: KmsKeyId,
+    RecipientPublicKey: Secret
+}
+
+
+@javadoc("Inputs for creating a KmsPublicKeyDiscovery Configuration. This is a DECRYPT ONLY configuration")
+structure KmsPublicKeyDiscoveryInput {
+    @required
+    @javadoc("AWS KMS key identifier belonging to the recipient")
+    recipientKmsIdentifier: KmsKeyId
+}
+
+@javadoc("Inputs for creating a KmsPrivateKeyToStaticPublicKey Configuration.")
+structure KmsPrivateKeyToStaticPublicKeyInput {
+    @required
+    @javadoc("AWS KMS Key Identifier belonging to the sender")
+    senderKmsIdentifier: KmsKeyId,
+    @required
+    @javadoc("Recipient configuration. This can be either a KMS key identifier or a raw public key")
+    recipientConfiguration: KmsRecipientConfiguration,
+}
+
+@javadoc("Inputs for creating a EphemeralPrivateKeyToStaticPublicKey Configuration.")
+structure EphemeralPrivateKeyToStaticPublicKeyInput {
+    @required
+    @javadoc("The recipient's public key")
+    recipientPublicKey: Secret,
+}
+
+@javadoc("Inputs for creating a PublicKeyDiscovery Configuration.")
+structure PublicKeyDiscoveryInput {
+    @required
+    @javadoc("The sender's private key")
+    senderStaticPrivateKey: Secret,
+}
+
+@javadoc("Inputs for creating a RawPrivateKeyToStaticPublicKey Configuration.")
+structure RawPrivateKeyToStaticPublicKeyInput {
+    @required
+    @javadoc("The sender's private key")
+    senderStaticPrivateKey: Secret,
+    @required
+    @javadoc("The recipient's public key")
+    recipientPublicKey: Secret,
+}
